Work on substitution lemma

theories/stlc.v
@@ -1,5 +1,6 @@
 From Coq Require Export List.
 Export ListNotations.
+Require Import Lia.
 
 
 (***********************************)
@@ -20,6 +21,13 @@ Module Type TY.
   Parameter ty : Set.
   Parameter ty_prp : ty.
   Parameter ty_arr : ty -> ty -> ty.
+
+  Parameter eqb_ty : ty -> ty -> bool.
+  Axiom eqb_ty_eq : forall A B, eqb_ty A B = true -> A = B.
+  Parameter is_ty_arr : ty -> option (ty * ty).
+  Axiom is_ty_arr_ty_arr : forall A B, is_ty_arr (ty_arr A B) = Some (A, B).
+  Axiom ty_arr_is_ty_arr :
+    forall A B t, is_ty_arr t = Some (A, B) -> t = ty_arr A B.
 End TY.
 
 (** Global notation declarations. *)
@@ -47,10 +55,49 @@ Module TyChurch <: TY.
     | tyc_prp : tyc
     | tyc_obj : tyc
     | tyc_arr : tyc -> tyc -> tyc.
+  Check tyc_rec.
 
   Definition ty := tyc.
   Definition ty_prp := tyc_prp.
   Definition ty_arr := tyc_arr.
+
+  Fixpoint eqb_ty S T :=
+    match S, T with
+    | tyc_arr A1 B1, tyc_arr A2 B2 => andb (eqb_ty A1 A2) (eqb_ty B1 B2)
+    | tyc_prp, tyc_prp => true
+    | tyc_obj, tyc_obj => true
+    | _, _ => false
+    end.
+  
+  Theorem eqb_ty_eq A B : eqb_ty A B = true -> A = B.
+  Proof.
+    generalize dependent B.
+    induction A; simpl in *; destruct B;
+      try discriminate; try reflexivity.
+    intros H. erewrite IHA1, IHA2.
+    - reflexivity.
+    - destruct (eqb_ty A2 B2); try reflexivity.
+      rewrite Bool.andb_false_r in H. discriminate.
+    - destruct (eqb_ty A1 B1); try reflexivity.
+      simpl in *. discriminate.
+  Qed.
+
+  Definition is_ty_arr t :=
+    match t with
+    | tyc_arr A B => Some (A, B)
+    | _ => None
+    end.
+
+  Theorem is_ty_arr_ty_arr A B :
+    is_ty_arr (ty_arr A B) = Some (A, B).
+  Proof. reflexivity. Qed.
+
+  Theorem ty_arr_is_ty_arr A B t :
+    is_ty_arr t = Some (A, B) -> t = ty_arr A B.
+  Proof.
+    intros H. destruct t; simpl in *; try discriminate.
+    injection H. intros. subst. reflexivity.
+  Qed.
 End TyChurch.
 
 Module TyChurchTheories.
@@ -137,6 +184,61 @@ Module Stlc (Ty : TY).
     | t_for c T : has_type c (tm_for T) <[ (T -> o) -> o ]>
     | t_ex  c T : has_type c (tm_ex  T) <[ (T -> o) -> o ]>.
 
+  Fixpoint type_check (c : context) (t : tm) : option ty :=
+    match t with
+    | tm_lvl n => nth_error c n
+    | tm_abs A t =>
+        match type_check (c ++ [A]) t with
+        | Some B => Some <[ A -> B ]>
+        | _ => None
+        end
+    | tm_app s t =>
+        match type_check c s, type_check c t with
+        | Some AR, Some A1 =>
+            match is_ty_arr AR with
+            | Some (A, B) => if eqb_ty A A1 then Some B else None
+            | _ => None
+            end
+        | _, _ => None
+        end
+    | tm_bot => Some ty_prp
+    | tm_top => Some ty_prp
+    | tm_and => Some <[ o -> o -> o ]>
+    | tm_or  => Some <[ o -> o -> o ]>
+    | tm_imp => Some <[ o -> o -> o ]>
+    | tm_for T => Some <[ (T -> o) -> o ]>
+    | tm_ex  T => Some <[ (T -> o) -> o ]>
+    end.
+
+  Theorem type_check_sound c t T :
+    type_check c t = Some T -> has_type c t T.
+  Proof.
+    generalize dependent c.
+    generalize dependent T.
+    induction t; intros T c TC;
+      try (simpl in TC; injection TC; intros <-; constructor).
+    - now constructor.
+    - remember (type_check c t1) as T1.
+      remember (type_check c t2) as T2.
+      simpl in TC. rewrite <- HeqT1, <- HeqT2 in TC.
+      destruct T1, T2; try discriminate.
+      remember (is_ty_arr t) as it.
+      destruct it eqn : E; try discriminate.
+      destruct p. symmetry in Heqit.
+      apply ty_arr_is_ty_arr in Heqit.
+      destruct (eqb_ty t3 t0) eqn : E1; [|discriminate].
+      apply eqb_ty_eq in E1.
+      injection TC. intros. subst.
+      eapply t_app.
+      + apply IHt1. symmetry. eassumption.
+      + apply IHt2. now symmetry.
+    - simpl in TC.
+      remember (type_check (c ++ [t]) t0) as H.
+      destruct H; try discriminate.
+      injection TC. intros <-.
+      constructor. apply IHt. now symmetry.
+  Qed.
+
   Notation "<| gam |- t : T |>" := (has_type gam t T)
     (at level 0, gam custom stlc_ty at level 200,
     t custom stlc_tm, T custom stlc_ty) : stlc_scope.
@@ -167,9 +269,57 @@ Module Stlc (Ty : TY).
     match t with
     | tm_lvl n => nth n l n
     | tm_app s t => tm_app (subst m l s) (subst m l t)
-    | tm_abs T t => tm_abs T (subst m (map (incr_bound m) l) t)
+    | tm_abs T t =>
+        tm_abs T (subst (m+1) ((map (incr_bound m) l) ++ [tm_lvl m]) t)
     | const => const
     end.
+
+  (** Examples *)
+  Compute fun i => subst 1 [<{ \: i, 1 }>; tm_lvl 0] <{ \: o, 1 0 }>.
+  Compute fun i => subst 2 [<{ \: i, 1 }>; tm_lvl 0] <{ \: o, 1 0 }>.
+  Compute fun i => subst 2 [<{ \: i, 0 1 }>] <{ \: o, 0 }>.
+  Compute fun i => subst 1 [<{ \: i, 0 1 }>] <{ \: o, 0 }>.
+  Compute fun i => subst 0 [<{ \: i, 0 0 }>] <{ \: o, 0 }>.
+  Compute fun i => subst 4 [tm_lvl 0; <{ \: i, 5 }>; tm_lvl 2] <{ 1 2 }>.
+  Compute fun i => subst 2 [tm_lvl 0; <{ \: i, 1 2 }>] <{ \: o, 1 }>.
+  Compute fun i =>
+    subst 0 [tm_lvl 0; tm_lvl 1; <{ \: i, 0 0 }>] <{ \: o, \: i, 2 2 }>.
+  Compute subst 0 [ tm_top ] <{ \: o, 1 }>.
+
+  Compute incr_bound 3 <{ \: o, \: o, 0 1 2 }>.
+
+  Theorem th C c t T : has_type C t T ->
+    has_type (C ++ [c]) (incr_bound (length C) t) T.
+  Proof.
+    intros HT.
+    generalize dependent T.
+    induction t; simpl; intros T HT.
+    - constructor. inversion HT. subst. rewrite <- H1.
+      destruct (PeanoNat.Nat.leb_spec0 (length C) n).
+      + generalize nth_error_None. intros N.
+        edestruct N as [_ N1]. rewrite N1.
+        * symmetry. now apply N.
+        * rewrite length_app. simpl. lia.
+      + apply PeanoNat.Nat.nle_gt in n0.
+        now rewrite nth_error_app1.
+    - inversion HT. subst. eapply t_app.
+      + apply IHt1. eassumption.
+      + now apply IHt2.
+    - inversion HT. subst.
+      constructor.
+
+    intros HT.
+    induction HT; simpl.
+    - constructor. rewrite <- H.
+      destruct (PeanoNat.Nat.leb_spec0 (length c0) n).
+      + generalize nth_error_None. intros N.
+        edestruct N as [_ N1]. rewrite N1.
+        * symmetry. now apply N.
+        * rewrite length_app. simpl. lia.
+      + apply PeanoNat.Nat.nle_gt in n0.
+        now rewrite nth_error_app1.
+    - constructor.
+
 
   Theorem has_type_subst C S T t s :
     Forall (fun si => has_type C si (S si)) s ->
@@ -190,7 +340,11 @@ Module Stlc (Ty : TY).
       + apply IHt1; eassumption.
       + auto.
     - inversion HT. subst. constructor.
+      replace (length C + 1) with (length (C ++ [t])).
       apply IHt.
+      + apply Forall_app. split.
+        * Print Forall.
+
 
   Theorem subst_lemma (A : ty) (t : tm) (s : list tm) (T : list ty) (S : tm -> ty) :
     Forall (fun si => <| T |- si : $(S si) |>) s -> (
@@ -208,3 +362,23 @@ Module Stlc (Ty : TY).
           rewrite nth_error_nil in H2. discriminate.
         * simpl in *.
 End Stlc.
+
+
+  Theorem th C t T n m : has_type C t T ->
+    n >= length C -> m >= length C ->
+    incr_bound n t = incr_bound m t.
+  Proof.
+    intros HT.
+    generalize dependent m. generalize dependent n.
+    induction HT; simpl; intros a b Ha Hb.
+    - assert (n < length c). {
+        generalize nth_error_None. intros N. edestruct N.
+        destruct (PeanoNat.Nat.leb_spec0 (length c) n).
+        - now rewrite H1 in H.
+        - lia.
+      }
+      destruct (PeanoNat.Nat.leb_spec0 a n), (PeanoNat.Nat.leb_spec0 b n); try reflexivity; lia.
+    - erewrite IHHT.
+      + reflexivity.
+      +
+
